finish proofs

src/crypto_foundations/primitives/symm_enc.lean
@@ -3,12 +3,10 @@ Copyright (c) 2023 Devon Tuma. All rights reserved.
 Released under Apache 2.0 license as described in the file LICENSE.
 Authors: Devon Tuma
 -/
-import computational_monads.distribution_semantics.monad
 import computational_monads.distribution_semantics.independence
 import computational_monads.constructions.uniform_select
 import computational_monads.constructions.product
 import computational_monads.support.prod
-import computational_monads.asymptotics.polynomial_time
 
 /-!
 # Symmetric-Key Encryption Schemes
@@ -67,19 +65,36 @@ section mgen_encrypt
 
 /-- Computation that given a message `m`, generates a key `k`, and then encrypts the message,
 returning both the generated message and the generated ciphertext `c`. -/
-@[inline, reducible]
-def mgen_encrypt (se_alg : symm_enc_alg M K C) (m_dist : oracle_comp uniform_selecting M) :
-  oracle_comp uniform_selecting (M × C) :=
+@[inline, reducible] def mgen_encrypt (se_alg : symm_enc_alg M K C)
+  (m_dist : oracle_comp uniform_selecting M) : oracle_comp uniform_selecting (M × C) :=
 do {m ← m_dist,
     k ← se_alg.keygen (),
     return (m, se_alg.encrypt (m, k))}
 
 variable (m_dist : oracle_comp uniform_selecting M)
 
-lemma eval_dist_mgen_encrypt_apply (x : M × C) :
-  ⁅= x | se_alg.mgen_encrypt m_dist⁆ =
-    ∑' (k : K), if x.2 = se_alg.encrypt (x.1, k)
-      then ⁅= x.1 | m_dist⁆ * ⁅= k | se_alg.keygen ()⁆ else 0 :=
+/-- support of `mgen_encrypt` is the union over possible messages and keys of the encryption. -/
+@[simp] lemma support_mgen_encrypt : (se_alg.mgen_encrypt m_dist).support =
+  ⋃ m ∈ m_dist.support, ⋃ k ∈ (se_alg.keygen ()).support, {(m, se_alg.encrypt (m, k))} :=
+by simp_rw [support_bind, support_return]
+
+lemma mem_support_mgen_encrypt_iff (m : M) (c : C) :
+  (m, c) ∈ (se_alg.mgen_encrypt m_dist).support ↔ m ∈ m_dist.support ∧
+    ∃ k ∈ (se_alg.keygen ()).support, se_alg.encrypt (m, k) = c :=
+by simp_rw [support_bind, support_return, set.mem_Union, set.mem_singleton_iff,
+  prod.eq_iff_fst_eq_snd_eq, exists_and_distrib_left, exists_prop, exists_eq_left', @eq_comm _ c]
+
+lemma exists_key_of_mem_support_mgen_encrypt (m : M) (c : C)
+  (h : (m, c) ∈ (se_alg.mgen_encrypt m_dist).support) :
+    ∃ k ∈ (se_alg.keygen ()).support, se_alg.encrypt (m, k) = c :=
+((se_alg.mem_support_mgen_encrypt_iff m_dist m c).1 h).2
+
+/-- The probability of getting a particular output `x` from `mgen_encrypt` is the sum over possible
+keys such that encrypt `x.1` to `x.2`, of the probability of getting that key,
+weighted by the probability of getting `x.1` from the message distribution. -/
+lemma eval_dist_mgen_encrypt_apply (x : M × C) : ⁅= x | se_alg.mgen_encrypt m_dist⁆ =
+  ∑' (k : K), if x.2 = se_alg.encrypt (x.1, k)
+    then ⁅= x.1 | m_dist⁆ * ⁅= k | se_alg.keygen ()⁆ else 0 :=
 begin
   simp only [←ennreal.tsum_mul_left, eval_dist_bind, eval_dist_bind_return, pmf.bind_apply,
     pmf.map_apply, mul_ite, mul_zero],
@@ -88,21 +103,9 @@ begin
   { simp_rw [prod.eq_iff_fst_eq_snd_eq, eq_self_iff_true, true_and] }
 end
 
-lemma eval_dist_fst_map_mgen_encrypt :
-  ⁅prod.fst <$> se_alg.mgen_encrypt m_dist⁆ = ⁅m_dist⁆ :=
+lemma eval_dist_fst_map_mgen_encrypt : ⁅prod.fst <$> se_alg.mgen_encrypt m_dist⁆ = ⁅m_dist⁆ :=
 by simp only [pmf.map_comp, eval_dist_map, eval_dist_bind, eval_dist_bind_return,
   pmf.map_bind, prod.fst_comp_mk, pmf.map_const, pmf.bind_pure]
-
-lemma mem_support_mgen_encrypt_iff (m : M) (c : C) :
-  (m, c) ∈ (se_alg.mgen_encrypt m_dist).support ↔
-    m ∈ m_dist.support ∧ ∃ k ∈ (se_alg.keygen ()).support, c = se_alg.encrypt (m, k) :=
-by simp_rw [support_bind, support_return, set.mem_Union, set.mem_singleton_iff,
-  prod.eq_iff_fst_eq_snd_eq, exists_and_distrib_left, exists_prop, exists_eq_left']
-
-lemma exists_key_of_mem_support_mgen_encrypt (m : M) (c : C)
-  (h : (m, c) ∈ (se_alg.mgen_encrypt m_dist).support) :
-    ∃ k ∈ (se_alg.keygen ()).support, c = se_alg.encrypt (m, k) :=
-((se_alg.mem_support_mgen_encrypt_iff m_dist m c).1 h).2
 
 end mgen_encrypt
 
@@ -117,13 +120,15 @@ def perfect_secrecy (se_alg : symm_enc_alg M K C) : Prop :=
 ∀ (m_dist : oracle_comp uniform_selecting M) (m : M) (c : C),
   indep_event (se_alg.mgen_encrypt m_dist) (prod.fst ⁻¹' {m}) (prod.snd ⁻¹' {c})
 
-theorem perfect_secrecy_iff : se_alg.perfect_secrecy ↔
-  ∀ (m_dist : oracle_comp uniform_selecting M) (m : M) (c : C),
-    ⁅= (m, c) | se_alg.mgen_encrypt m_dist⁆ =
-      ⁅= m | m_dist⁆ * ⁅= c | prod.snd <$> se_alg.mgen_encrypt m_dist⁆ :=
+/-- Restate perfect secrecy in terms of explicit probabilities instead of indepent events.
+A symmetric encryption algorithm has perfect secrecy iff the probability of getting a given
+message-ciphertext after generating a key and encrypting is the probability of drawing the message
+times the probability of getting that ciphertext from any message, for any message distribution. -/
+theorem perfect_secrecy_iff : se_alg.perfect_secrecy ↔ ∀ (m_dist : oracle_comp uniform_selecting M)
+  (m : M) (c : C), ⁅= (m, c) | se_alg.mgen_encrypt m_dist⁆ =
+    ⁅= m | m_dist⁆ * ⁅= c | prod.snd <$> se_alg.mgen_encrypt m_dist⁆ :=
 begin
   refine forall_congr (λ m_dist, (forall_congr (λ m, forall_congr (λ c, _)))),
-  rw [indep_event_iff],
   have this : prod.fst ⁻¹' {m} ∩ prod.snd ⁻¹' {c} = ({(m, c)} : set (M × C)),
   by {ext x, simp only [prod.eq_iff_fst_eq_snd_eq, set.mem_inter_iff,
     set.mem_preimage, set.mem_singleton_iff]},
@@ -138,13 +143,13 @@ variables [fintype M] [fintype K] [fintype C]
 include hmk hkc
 
 /-- If all spaces have the same size we can get bijectivity of encrypt not just injectivity. -/
-lemma encrypt_bijective (k : K) (hk : k ∈ (se_alg.keygen ()).support) :
+lemma encrypt_bijective_of_equal_card (k : K) (hk : k ∈ (se_alg.keygen ()).support) :
   (λ m, se_alg.encrypt (m, k)).bijective :=
 (fintype.bijective_iff_injective_and_card _).2
   ⟨se_alg.encrypt_injective k hk, hmk.trans hkc⟩
 
 /-- If all spaces have the same size we can get bijectivity of decrypt not just surjectivity. -/
-lemma decrypt_bijective (k : K) (hk : k ∈ (se_alg.keygen ()).support) :
+lemma decrypt_bijective_of_equal_card (k : K) (hk : k ∈ (se_alg.keygen ()).support) :
   (λ c, se_alg.decrypt (c, k)).bijective :=
 (fintype.bijective_iff_surjective_and_card _).2
   ⟨se_alg.decrypt_surjective k hk, symm $ hmk.trans hkc⟩
@@ -152,51 +157,132 @@ lemma decrypt_bijective (k : K) (hk : k ∈ (se_alg.keygen ()).support) :
 /-- If all spaces are the same size then encryption and decryption are also left inverses. -/
 lemma left_inverse_encrypt_decrypt : ∀ k ∈ (se_alg.keygen ()).support,
   function.left_inverse (λ m, se_alg.encrypt (m, k)) (λ c, se_alg.decrypt (c, k)) :=
-λ k hk c, (se_alg.decrypt_bijective hmk hkc k hk).1 (by simp only [se_alg.complete _ k hk])
+λ k hk c, (se_alg.decrypt_bijective_of_equal_card hmk hkc k hk).1
+  (by simp only [se_alg.complete _ k hk])
 
-lemma encrypt_decrypt_eq_iff (c : C) (k k' : K) (hk : k ∈ (se_alg.keygen ()).support) :
-  se_alg.encrypt (se_alg.decrypt (c, k), k') = c ↔ k' = k :=
+/-- Reverse version of completeness, i.e. encrypting a decryption gives the initial value. -/
+lemma complete' (c : C) (k : K) (hk : k ∈ (se_alg.keygen ()).support) :
+  se_alg.encrypt (se_alg.decrypt (c, k), k) = c :=
+se_alg.left_inverse_encrypt_decrypt hmk hkc k hk c
+
+section perfect_secrecy
+
+/-- Given perfect secrecy and matching cardinatlities, every message-ciphertext pair must
+give rise to a key that encrypts that message to that ciphertext. -/
+theorem exists_unique_key_of_perfect_secrecy (h : se_alg.perfect_secrecy) (m : M) (c : C) :
+  ∃! k, k ∈ (se_alg.keygen ()).support ∧ se_alg.encrypt (m, k) = c :=
 begin
-  refine ⟨λ hk, _, λ hk, _⟩,
-  {
-    sorry,
+  have hmc : ∀ m c, ∃ k, k ∈ (se_alg.keygen ()).support ∧ se_alg.encrypt (m, k) = c,
+  { intros m c,
+    haveI : nonempty M := ⟨m⟩, -- Can't represent a uniform distribution on an empty type.
+    suffices : 0 < ⁅= (m, c) | se_alg.mgen_encrypt ($ᵗ M)⁆,
+    { rw [eval_dist_pos_iff_mem_support] at this,
+      obtain ⟨k, hk, hk'⟩ := se_alg.exists_key_of_mem_support_mgen_encrypt ($ᵗ M) m c this,
+      refine ⟨k, hk, hk'⟩ },
+    {
+      have this := (se_alg.perfect_secrecy_iff.1 h) ($ᵗ M) m c,
+    simp_rw [this, ennreal.mul_pos_iff, eval_dist_pos_iff_mem_support,
+      mem_support_uniform_select_fintype, mem_support_map_snd_iff, mem_support_mgen_encrypt_iff,
+      mem_support_uniform_select_fintype M, true_and, exists_prop],
+    obtain ⟨k, hk⟩ := (se_alg.keygen ()).support_nonempty,
+    exact ⟨se_alg.decrypt (c, k), k, hk, se_alg.left_inverse_encrypt_decrypt hmk hkc k hk c⟩,
+    }
   },
+  have : (λ k, se_alg.encrypt (m, k)).bijective,
   {
-    rw [hk],
-    apply left_inverse_encrypt_decrypt; assumption
-  }
+    rw fintype.bijective_iff_surjective_and_card,
+    refine ⟨λ c, _, hkc⟩,
+    have := hmc m c,
+    refine let ⟨k, _, hk⟩ := this in ⟨k, hk⟩,
+  },
+
+  refine exists_unique_of_exists_of_unique (hmc m c) _,
+
+  refine λ k k' hk hk', _,
+  have hkk' := hk.2.trans hk'.2.symm,
+  refine this.1 hkk',
 end
+
+/-- Given perfect secrecy and matching cardinatlities, the keygen function must include
+all possible keys in its set of possible outputs. -/
+lemma support_keygen_of_perfect_secrecy (h : se_alg.perfect_secrecy) :
+  (se_alg.keygen ()).support = set.univ :=
+begin
+  refine set.to_finset_eq_univ.1 (finset.eq_univ_of_card _ $ antisymm (finset.card_le_univ _) _),
+  by_cases hM : nonempty M,
+  { refine hM.elim (λ m, _),
+    calc fintype.card K = fintype.card C : hkc
+      ... ≤ ((λ k, se_alg.encrypt (m, k)) '' (se_alg.keygen ()).support).to_finset.card :
+        finset.card_le_of_subset (λ c hc, set.mem_to_finset.2 ((set.mem_image _ _ _).2 $
+          exists_of_exists_unique (se_alg.exists_unique_key_of_perfect_secrecy hmk hkc h m c)))
+      ... ≤ (se_alg.keygen ()).support.to_finset.card :
+        by simpa only [set.to_finset_image] using finset.card_image_le },
+  { simpa only [← hmk, @fintype.card_eq_zero M _ (not_nonempty_iff.1 hM)] using zero_le' }
+end
+
+/-- Given perfect secrecy and matching cardinality, all keys are possible outputs of `keygen`. -/
+lemma mem_support_keygen (h : se_alg.perfect_secrecy) (k : K) : k ∈ (se_alg.keygen ()).support :=
+(se_alg.support_keygen_of_perfect_secrecy hmk hkc h).symm ▸ set.mem_univ k
+
+/-- If all spaces have the same size we can get bijectivity of encrypt not just injectivity,
+where encryption is viewed as a function on keys with a fixed message. -/
+lemma encrypt_key_bijective_of_perfect_secrecy (h : se_alg.perfect_secrecy) (m : M) :
+  (λ k, se_alg.encrypt (m, k)).bijective :=
+(function.bijective_iff_exists_unique _).2 $
+  λ c, let ⟨k, hk, h'⟩ := se_alg.exists_unique_key_of_perfect_secrecy hmk hkc h m c
+  in ⟨k, hk.2, λ k' hk', h' k' ⟨se_alg.mem_support_keygen hmk hkc h k', hk'⟩⟩
+
+/-- If all spaces have the same size we can get bijectivity of encrypt not just injectivity,
+where decryption is viewed as a function on keys with a fixed ciphertext. -/
+lemma decrypt_key_bijective_of_perfect_secrecy (h : se_alg.perfect_secrecy) (c : C) :
+  (λ k, se_alg.decrypt (c, k)).bijective :=
+begin
+  refine (function.bijective_iff_exists_unique _).2 (λ m, _),
+  obtain ⟨k, hk, h'⟩ := se_alg.exists_unique_key_of_perfect_secrecy hmk hkc h m c,
+  exact ⟨k, hk.2 ▸ se_alg.complete m k hk.1, λ k' hk', h' k' ⟨se_alg.mem_support_keygen
+    hmk hkc h k', hk' ▸ se_alg.complete' hmk hkc c k' (se_alg.mem_support_keygen hmk hkc h k')⟩⟩,
+end
+
+lemma decrypt_encrypt_eq_iff_of_perfect_secrecy (h : se_alg.perfect_secrecy) (m : M) (k k' : K) :
+  se_alg.decrypt (se_alg.encrypt (m, k), k') = m ↔ k = k' :=
+have hk : k ∈ (se_alg.keygen ()).support := (se_alg.mem_support_keygen hmk hkc h k),
+have hk' : k' ∈ (se_alg.keygen ()).support := (se_alg.mem_support_keygen hmk hkc h k'),
+⟨λ h', (se_alg.encrypt_key_bijective_of_perfect_secrecy hmk hkc h m).1
+  ((se_alg.decrypt_bijective_of_equal_card hmk hkc k' hk').1
+  (h'.trans (se_alg.complete m k' hk').symm)), λ h', h' ▸ se_alg.complete m k hk⟩
+
+lemma encrypt_decrypt_eq_iff_of_perfect_secrecy (h : se_alg.perfect_secrecy) (c : C) (k k' : K) :
+  se_alg.encrypt (se_alg.decrypt (c, k), k') = c ↔ k = k' :=
+have hk : k ∈ (se_alg.keygen ()).support := (se_alg.mem_support_keygen hmk hkc h k),
+have hk' : k' ∈ (se_alg.keygen ()).support := (se_alg.mem_support_keygen hmk hkc h k'),
+⟨λ h', (se_alg.decrypt_key_bijective_of_perfect_secrecy hmk hkc h c).1
+  ((se_alg.encrypt_bijective_of_equal_card hmk hkc k' hk').1
+  (h'.trans (se_alg.complete' hmk hkc c k' hk').symm)), λ h', h' ▸ se_alg.complete' hmk hkc c k hk⟩
 
 lemma eval_dist_key_eq_eval_dist_cipher_of_perfect_secrecy (h : se_alg.perfect_secrecy)
   (m_dist : oracle_comp uniform_selecting M) (k : K) (c : C)
   (h' : se_alg.decrypt (c, k) ∈ m_dist.support) :
   ⁅= k | se_alg.keygen ()⁆ = ⁅= c | prod.snd <$> se_alg.mgen_encrypt m_dist⁆ :=
 begin
-  suffices : ⁅= se_alg.decrypt (c, k) | m_dist⁆ * ⁅= k | se_alg.keygen ()⁆ =
-    ⁅= se_alg.decrypt (c, k) | m_dist⁆ * ⁅= c | prod.snd <$> se_alg.mgen_encrypt m_dist⁆,
-  from begin
-    rwa [ennreal.mul_eq_mul_left _ (pmf.apply_ne_top _ _)] at this,
-    rw [eval_dist_ne_zero_iff_mem_support],
-    exact h',
-  end,
   let m := se_alg.decrypt (c, k),
+  suffices : ⁅= m | m_dist⁆ * ⁅= k | se_alg.keygen ()⁆ =
+    ⁅= m | m_dist⁆ * ⁅= c | prod.snd <$> se_alg.mgen_encrypt m_dist⁆,
+  from (ennreal.mul_eq_mul_left (eval_dist_ne_zero_of_not_mem_support h') (pmf.apply_ne_top _ _)).1 this,
   calc ⁅= m | m_dist⁆ * ⁅= k | se_alg.keygen ()⁆ =
     ⁅= (m, k) | m_dist ×ₘ se_alg.keygen ()⁆ : by rw [eval_dist_product_apply]
     ... = ⁅= (m, c) | (λ (x : M × K), (x.1, se_alg.encrypt (x.1, x.2))) <$> (m_dist ×ₘ se_alg.keygen ())⁆ :
     begin
-      refine symm _,
-      by_cases hkk : k ∈ (se_alg.keygen ()).support,
+      refine symm (eval_dist_map_apply_eq_single' _ _ _ _ _ _),
       {
-        apply eval_dist_map_apply_eq_single,
-        refine set.ext (λ x, x.rec $ λ m' k', _),
-        simp only [prod.eq_iff_fst_eq_snd_eq, set.mem_preimage, set.mem_singleton_iff, and.congr_right_iff],
-        intro h,
-        simp only [h, m],
-        apply encrypt_decrypt_eq_iff; assumption
-
+        simpa only [prod.mk.inj_iff, eq_self_iff_true, true_and] using
+          se_alg.complete' hmk hkc c k (se_alg.mem_support_keygen hmk hkc h k),
       },
       {
-        sorry
+        refine λ x hx hxm, _,
+        simp only [prod.eq_iff_fst_eq_snd_eq] at hxm ⊢,
+        refine ⟨hxm.1, _⟩,
+        have : se_alg.encrypt (m, x.snd) = c := hxm.1 ▸ hxm.2,
+        exact symm ((se_alg.encrypt_decrypt_eq_iff_of_perfect_secrecy hmk hkc h _ _ _).1 this),
       }
     end
     ... = ⁅= (m, c) | se_alg.mgen_encrypt m_dist⁆ :
@@ -206,27 +292,6 @@ begin
       (se_alg.perfect_secrecy_iff.1 h) m_dist m c
 end
 
-theorem exists_key_of_perfect_secrecy (h : se_alg.perfect_secrecy) (m : M) (c : C) :
-  ∃ k ∈ (se_alg.keygen ()).support, c = se_alg.encrypt (m, k) :=
-begin
-  haveI : nonempty M := ⟨m⟩, -- Can't represent a uniform distribution on an empty type.
-  suffices : 0 < ⁅= (m, c) | se_alg.mgen_encrypt ($ᵗ M)⁆,
-  { rw [eval_dist_pos_iff_mem_support] at this,
-    exact se_alg.exists_key_of_mem_support_mgen_encrypt ($ᵗ M) m c this },
-  { have this := (se_alg.perfect_secrecy_iff.1 h) ($ᵗ M) m c,
-    simp_rw [this, ennreal.mul_pos_iff, eval_dist_pos_iff_mem_support,
-      mem_support_uniform_select_fintype, mem_support_map_snd_iff, mem_support_mgen_encrypt_iff,
-      mem_support_uniform_select_fintype M, true_and, exists_prop, @eq_comm _ c],
-    obtain ⟨k, hk⟩ := (se_alg.keygen ()).support_nonempty,
-    exact ⟨se_alg.decrypt (c, k), k, hk, se_alg.left_inverse_encrypt_decrypt hmk hkc k hk c⟩ }
-end
-
-theorem key_unique_of_perfect_secrecy (h : se_alg.perfect_secrecy) (m : M) (k k' : K)
-  (hk : k ∈ (se_alg.keygen ()).support) (hk' : k' ∈ (se_alg.keygen ()).support)
-  (h : se_alg.encrypt (m, k) = se_alg.encrypt (m, k')) : k = k' :=
-begin
-  sorry
-end
 
 /-- Assuming that the message, key, and ciphertext spaces all have the same size,
 any system with perfect secrecy must generate keys uniformly at random. -/
@@ -247,16 +312,18 @@ calc ⁅= k | se_alg.keygen ()⁆ =
   ... = (fintype.card C)⁻¹ : by rw [pmf.tsum_coe, mul_one]
   ... = (fintype.card K)⁻¹ : by rw hkc
 
-lemma perfect_secrecy_iff_of_equal_card [nonempty M] [nonempty C] :
+/-- Given that all spaces have the same cardinality, perfect secrecy holds iff:
+1. `keygen` chooses keys uniformly at random.
+2. for every message `m` and ciphertext `c`, there is a unique key encrypting `m` to `c`.
+In particular this will be used to show perfect secrecy of the one-time pad.-/
+theorem perfect_secrecy_iff_of_equal_card [nonempty M] [nonempty C] :
   se_alg.perfect_secrecy ↔
   (∀ k, ⁅= k | se_alg.keygen ()⁆ = (fintype.card K)⁻¹) ∧
-    (∀ m c, ∃! k, k ∈ (se_alg.keygen ()).support ∧ c = se_alg.encrypt (m, k)) :=
+    (∀ m c, ∃! k, k ∈ (se_alg.keygen ()).support ∧ se_alg.encrypt (m, k) = c) :=
 begin
   split,
-  { refine λ h, ⟨se_alg.eval_dist_keygen_eq_uniform_of_perfect_secrecy hmk hkc h, λ m c, _⟩,
-    obtain ⟨k, hk, hkm⟩ := se_alg.exists_key_of_perfect_secrecy hmk hkc h m c,
-    exact ⟨k, ⟨hk, hkm⟩, λ k' hk', se_alg.key_unique_of_perfect_secrecy
-      hmk hkc h m k' k hk'.1 hk (hk'.2.symm.trans hkm)⟩ },
+  { refine λ h, ⟨se_alg.eval_dist_keygen_eq_uniform_of_perfect_secrecy hmk hkc h,
+      λ m c, se_alg.exists_unique_key_of_perfect_secrecy hmk hkc h m c⟩ },
   { rw [perfect_secrecy_iff],
     rintros ⟨h_keygen, h_encrypt⟩ m_dist m c,
     obtain ⟨k, ⟨⟨hkₛ, rfl⟩, hk⟩⟩ := h_encrypt m c,
@@ -268,7 +335,7 @@ begin
           refine tsum_congr (λ k', symm _),
           by_cases hk0 : k' ∈ (se_alg.keygen ()).support,
           { exact ite_eq_iff'.2 ⟨λ hk'', by rw [hk'', eq_self_iff_true, if_true], λ hkn, symm $
-              ite_eq_right_iff.2 $ λ hk'', false.elim (hkn (hk k' ⟨hk0, hk''⟩).symm)⟩ },
+              ite_eq_right_iff.2 $ λ hk'', false.elim (hkn (hk k' ⟨hk0, hk''.symm⟩).symm)⟩ },
           { simp_rw [(eval_dist_eq_zero_iff_not_mem_support _ _).2 hk0, mul_zero, if_t_t] }
         end
       ... = if k = k then ⁅= m | m_dist⁆ * ⁅= k | se_alg.keygen ()⁆ else 0 :
@@ -283,7 +350,7 @@ begin
           obtain ⟨k', hks', hke'⟩ := h_encrypt m' (se_alg.encrypt (m, k)),
           refine trans (tsum_eq_single k' $ λ kd hkd, _) _,
           { by_cases hkds : kd ∈ (se_alg.keygen ()).support,
-            { exact ite_eq_right_iff.2 (λ hkkd, false.elim (hkd $ hke' kd ⟨hkds, hkkd⟩)) },
+            { exact ite_eq_right_iff.2 (λ hkkd, false.elim (hkd $ hke' kd ⟨hkds, hkkd.symm⟩)) },
             { simp_rw [(eval_dist_eq_zero_iff_not_mem_support _ _).2 hkds, mul_zero, if_t_t] } },
           { simp_rw [hks'.2, eq_self_iff_true, if_true, h_keygen] }
         end
@@ -296,6 +363,8 @@ begin
         end
   }
 end
+
+end perfect_secrecy
 
 end equal_card
 
